More progress in the flow-interface version of lookup.

concurrency/puretree.v
@@ -277,3 +277,201 @@ Proof.
 Qed.
 
 Arguments range_incl _ _ : simpl nomatch.
+
+Section Trees.
+
+  Variable V : Type.
+  Variable default: V.
+
+  Definition key := Z.
+
+  Inductive tree : Type :=
+  | E : tree
+  | T: tree -> key -> V -> tree -> tree.
+
+  Inductive In (k : key) : tree -> Prop :=
+  | InRoot l r x v:  (k = x) -> In k (T l x v r )
+  | InLeft l r x v': In k l -> In k (T l x v' r)
+  | InRight l r x v': In k r -> In k (T l x v' r).
+
+  Definition lt (t: tree) (k: key) := forall x : key, In x t -> k < x .
+  Definition gt (t: tree) (k: key) := forall x : key, In x t -> k > x .
+
+  Inductive sorted_tree : tree -> Prop :=
+  | Sorted_Empty : sorted_tree E
+  | Sorted_Tree x v l r : sorted_tree l -> sorted_tree r ->
+                          gt l x -> lt r x -> sorted_tree (T l x v r ).
+
+  Fixpoint lookup (x: key) (t : tree) : V :=
+    match t with
+    | E => default
+    | T tl k v tr => if x <? k then lookup x tl
+                     else if k <? x then lookup x tr
+                          else v
+    end.
+
+  Fixpoint insert (x: key) (v: V) (s: tree) : tree :=
+    match s with
+    | E => T E x v E
+    | T a y v' b => if  x <? y then T (insert x v a) y v' b
+                    else if y <? x then T a y v' (insert x v b)
+                         else T a x v b
+    end.
+
+  Fixpoint pushdown_left (a: tree) (bc: tree) : tree :=
+    match bc with
+    | E => a
+    | T b y vy c => T (pushdown_left a b) y vy c
+    end.
+
+  Fixpoint delete (x: key) (s: tree) : tree :=
+    match s with
+    | E => E
+    | T a y v' b => if  x <? y then T (delete x a) y v' b
+                    else if y <? x then T a y v' (delete x b)
+                         else pushdown_left a b
+    end.
+
+  Definition insert_seq (s: list (key * V)) (tr: tree) :=
+    fold_left (fun t x => insert (fst x) (snd x) t) s tr.
+
+  Definition insert_seq_opt (b: bool) (v: V) l1 l2 :=
+    if b
+    then insert_seq (l1 ++ (1, v) :: l2) E
+    else insert_seq (l1 ++ l2) E.
+
+  Lemma value_in_tree: forall x v k (t: tree),
+      In k (insert x v t) -> (x = k) \/ In k t.
+  Proof.
+    intros. induction t; simpl in H. 1: inversion H; subst; auto.
+    destruct (x <? k0) eqn: Heqn.
+    - inversion H; subst.
+      + right. apply InRoot. auto.
+      + specialize (IHt1 H1). destruct IHt1. left. auto. right. apply InLeft. auto.
+      + right. apply InRight. auto.
+    - destruct (k0 <? x) eqn: Heqn'.
+      + inversion H; subst.
+        * right. apply InRoot. auto.
+        * right. apply InLeft. auto.
+        * specialize (IHt2 H1). destruct IHt2. left. auto. right. apply InRight. auto.
+      + assert (k0 = x).
+        { apply Z.ltb_nlt in Heqn'. apply Z.ltb_nlt in Heqn. lia. }
+        subst. right. inversion H; subst.
+        * apply InRoot. auto.
+        * apply InLeft. auto.
+        * apply InRight. auto.
+  Qed.
+
+  Lemma insert_sorted : forall x v (t: tree),
+      sorted_tree t -> sorted_tree (insert x v t).
+  Proof.
+    intros. induction t.
+    - simpl. apply Sorted_Tree; auto; [unfold gt | unfold lt]; intros; easy.
+    - simpl. destruct (x <? k)  eqn: Heqn.
+      + constructor.
+        * apply IHt1. inversion H; auto.
+        * inversion H; auto.
+        * unfold gt. intros. apply value_in_tree in H0. destruct H0. subst.
+          apply Z.ltb_lt in Heqn. lia.  inversion H;subst. auto.
+        * unfold lt. intros. inversion H; subst. auto.
+      + destruct (k <? x) eqn: Heqn'.
+        * apply Sorted_Tree.
+          -- inversion H; subst. auto.
+          -- apply IHt2. inversion H. auto.
+          -- unfold gt. intros. inversion H; subst. auto.
+          -- unfold lt. intros. apply value_in_tree in H0. destruct H0.
+             ++ subst. apply Z.ltb_lt in Heqn'. lia.
+             ++ inversion H; subst. auto.
+        * assert (k = x).
+          {apply Z.ltb_nlt in Heqn'. apply Z.ltb_nlt in Heqn. lia. }
+          subst. apply Sorted_Tree; inversion H; subst; auto.
+  Qed.
+
+  Lemma insert_seq_sorted: forall l tr,
+      sorted_tree tr -> sorted_tree (insert_seq l tr).
+  Proof.
+    induction l. intros. 1: now simpl.
+    change (a :: l) with ([a] ++ l). unfold insert_seq in *.
+    intros. rewrite fold_left_app. fold insert_seq. apply IHl. simpl.
+    now apply insert_sorted.
+  Qed.
+
+  Lemma insert_seq_assoc: forall k v l,
+      insert k v (insert_seq l E) = insert_seq (l ++ [(k, v)]) E.
+  Proof.
+    intros.
+    change (insert k v (insert_seq l E)) with (insert_seq [(k ,v)] (insert_seq l E)).
+    unfold insert_seq. now rewrite <- fold_left_app.
+  Qed.
+
+  Lemma insert_seq_opt_sorted: forall b v l1 l2,
+      sorted_tree (insert_seq_opt b v l1 l2).
+  Proof. intros. destruct b; simpl; apply insert_seq_sorted; constructor. Qed.
+
+  Lemma insert_seq_opt_assoc:
+    forall (k : key) (v : V) (b : bool) (v0 : V) (l1 l2 : list (key * V)),
+      insert k v (insert_seq_opt b v0 l1 l2) = insert_seq_opt b v0 l1 (l2 ++ [(k, v)]).
+  Proof.
+    intros. destruct b; unfold insert_seq_opt; rewrite insert_seq_assoc.
+    - f_equal. rewrite <- app_assoc. f_equal.
+    - f_equal. rewrite <- app_assoc. easy.
+  Qed.
+
+  Lemma pushdown_left_In: forall (t1 t2: tree) (x: key),
+      In x (pushdown_left t1 t2) -> In x t1 \/ In x t2.
+  Proof.
+    intros. revert t2 H. induction t2; intros; simpl in *; auto. inversion H; subst.
+    - right. now apply InRoot.
+    - apply IHt2_1 in H1. destruct H1; [left | right]; auto. now apply InLeft.
+    - right. now apply InRight.
+  Qed.
+
+  Lemma delete_In: forall (x: key) (t: tree) (y: key), In y (delete x t) -> In y t.
+  Proof.
+    intros. revert t H. induction t; intros; simpl in *; auto. destruct (x <? k).
+    - inversion H; subst;
+        try ((now apply InLeft) || (now apply InRoot) || (now apply InRight)).
+      apply IHt1 in H1. now apply InLeft.
+    - destruct (k <? x).
+      + inversion H; subst;
+          try ((now apply InLeft) || (now apply InRoot) || (now apply InRight)).
+        apply IHt2 in H1. now apply InRight.
+      + apply pushdown_left_In in H. destruct H; [apply InLeft | apply InRight]; easy.
+  Qed.
+
+  Lemma pushdown_left_sorted: forall (t1 t2: tree),
+      sorted_tree t1 -> sorted_tree t2 -> (forall x y, In x t1 -> In y t2 -> x < y) ->
+      sorted_tree (pushdown_left t1 t2).
+  Proof.
+    intros. revert t2 H0 H1. induction t2; intros; simpl in H0 |-* ; auto.
+    inversion H0; subst; constructor; auto.
+    - apply IHt2_1; auto. intros. apply H1; auto. now apply InLeft.
+    - intros z ?. apply pushdown_left_In in H2. destruct H2.
+      + apply Z.lt_gt, H1; auto. now apply InRoot.
+      + now specialize (H8 _ H2).
+  Qed.
+
+  Lemma delete_sorted: forall (x: key) (t: tree),
+      sorted_tree t -> sorted_tree (delete x t).
+  Proof.
+    intros. revert t H. induction t; intros; simpl; auto. inversion H; subst.
+    destruct (x <? k) eqn: ?.
+    - apply Z.ltb_lt in Heqb. constructor; auto. intros y ?.
+      apply delete_In in H0. now apply H6.
+    - apply Z.ltb_ge in Heqb. destruct (k <? x) eqn: ?.
+      + apply Z.ltb_lt in Heqb0. constructor; auto. intros y ?.
+        apply delete_In in H0. now apply H7.
+      + apply pushdown_left_sorted; auto. intros y z ? ?.
+        apply H6 in H0. apply H7 in H1. lia.
+  Qed.
+
+End Trees.
+
+Arguments E {_}.
+Arguments T {_}.
+Arguments sorted_tree {_}.
+Arguments lookup {_}.
+Arguments insert {_}.
+Arguments pushdown_left {_}.
+Arguments delete {_}.
+Arguments insert_seq_opt {_}.
