concurrency/verif_bst_flows.v
@@ -15,7 +15,8 @@ Definition bst_inset_flowint := inset_flowint TreeNode Z.
 
 Definition inset_global_inv (root: TreeNode) (NS: list TreeNode)
            (Iset: bst_inset_flowint) : Prop :=
-  keyset_global_inv root Iset /\ list_to_set (map key_tn NS) ⊆ KS.
+  keyset_global_inv root Iset /\ list_to_set (map key_tn NS) ⊆ KS /\
+  (forall n, n ∈ domm Iset -> n <> root -> inf Iset n = ∅).
 
 Definition gmap_sub `{Countable K} {A} (s1 s2: gmap K A): Prop :=
   forall k a, s1 !! k = Some a -> s2 !! k = Some a.
@@ -36,13 +37,13 @@ Proof.
 Qed.
 
 Definition splitLeft (mulst: gmap Z nat) (e: Z): gmap Z nat :=
-  list_to_map (List.filter (fun zn => (fst zn) <? e) (map_to_list mulst)).
+  list_to_map (List.filter (fun zn => e >? (fst zn)) (map_to_list mulst)).
 
 Lemma nzmap_left_wf: forall m e,  nzmap_wf m -> nzmap_wf (splitLeft m e).
 Proof. intros. apply nzmap_subset_wf with m; auto. apply split_filter_sub. Qed.
 
 Definition splitRight (mulst: gmap Z nat) (e: Z): gmap Z nat :=
-  list_to_map (List.filter (fun zn => (fst zn) >? e) (map_to_list mulst)).
+  list_to_map (List.filter (fun zn => e <? (fst zn)) (map_to_list mulst)).
 
 Lemma nzmap_right_wf: forall m e,  nzmap_wf m -> nzmap_wf (splitRight m e).
 Proof. intros. apply nzmap_subset_wf with m; auto. apply split_filter_sub. Qed.
@@ -56,6 +57,45 @@ Definition split_right (s: K_multiset Z) (e: Z): K_multiset Z :=
   let (m, Hm) := s in
   NZMap (splitRight m e)
         (bool_decide_pack _ (nzmap_right_wf m e (bool_decide_unpack _ Hm))).
+
+Lemma filter_fst: forall {A B: Type} (f: A -> bool) (l: list (A * B)),
+    (List.filter (fun zn => f zn.1) l).*1 = List.filter f l.*1.
+Proof.
+  intros. induction l; simpl; auto.
+  destruct (f a.1); [rewrite fmap_cons |]; now rewrite IHl.
+Qed.
+
+Lemma split_right_lookup: forall s e i a,
+    (split_right s e) !! i = Some a <-> (s !! i = Some a /\ i > e).
+Proof.
+  intros. split; intros; unfold lookup in *; destruct s; simpl in *.
+  - unfold splitRight in H. apply elem_of_list_to_map_2 in H.
+    apply elem_of_list_In in H. apply filter_In in H. simpl in H. destruct H.
+    rewrite <- elem_of_list_In in H. apply elem_of_map_to_list in H. split; auto.
+    apply Zlt_is_lt_bool in H0. lia.
+  - unfold splitRight. apply elem_of_list_to_map.
+    + rewrite filter_fst. rewrite NoDup_ListNoDup. apply List.NoDup_filter.
+      rewrite <- NoDup_ListNoDup. apply NoDup_fst_map_to_list.
+    + rewrite elem_of_list_In. rewrite filter_In. simpl. split.
+      * rewrite <- elem_of_list_In. now rewrite elem_of_map_to_list.
+      * rewrite <- Zlt_is_lt_bool. lia.
+Qed.
+
+Lemma split_left_lookup: forall s e i a,
+    (split_left s e) !! i = Some a <-> (s !! i = Some a /\ i < e).
+Proof.
+  intros. split; intros; unfold lookup in *; destruct s; simpl in *.
+  - unfold splitLeft in H. apply elem_of_list_to_map_2 in H.
+    apply elem_of_list_In in H. apply filter_In in H. simpl in H. destruct H.
+    rewrite <- elem_of_list_In in H. apply elem_of_map_to_list in H. split; auto.
+    apply Zgt_is_gt_bool in H0. lia.
+  - unfold splitLeft. apply elem_of_list_to_map.
+    + rewrite filter_fst. rewrite NoDup_ListNoDup. apply List.NoDup_filter.
+      rewrite <- NoDup_ListNoDup. apply NoDup_fst_map_to_list.
+    + rewrite elem_of_list_In. rewrite filter_In. simpl. split.
+      * rewrite <- elem_of_list_In. now rewrite elem_of_map_to_list.
+      * rewrite <- Zgt_is_gt_bool. lia.
+Qed.
 
 Definition inset_edgeFn (x y: TreeNode): K_multiset Z -> K_multiset Z :=
   fun s => if (val_eqb x.(addr_tn) y.(addr_tn) || val_eqb y.(addr_tn) nullval)%bool
@@ -203,18 +243,41 @@ Proof.
     rewrite tree_rep_cons. Exists nI nS Cl1 Cl2. entailer !.
 Qed.
 
+Lemma tree_rep_root_no_parent: forall root l C1 C2,
+    !!(pc_global_inv root l C1) && tree_rep l C1 C2 |--
+          !! (forall x, In x l -> left_tn x <> addr_tn root /\
+                                  right_tn x <> addr_tn root).
+Proof.
+  intros. Intros. eapply derives_trans. 1: apply tree_rep_impl_pc_tree_rep.
+  sep_apply (pc_tree_rep_root_no_parent root); auto. entailer !.
+Qed.
+
 Lemma node_rep_valid_ptr: forall n nI nS,
     node_rep n nI nS |-- valid_pointer (addr_tn n).
 Proof. intros. unfold node_rep. entailer !. Qed.
+
+Lemma tree_rep_local_inv: forall l,
+    iter_sepcon (fun x => node_rep x.1 x.2.1 x.2.2) l |--
+                !! (forall x, In x l -> pc_local_inv x.1 x.2.1 /\
+                                        inset_local_inv x.1 x.2.2).
+Proof.
+  intros. induction l.
+  - apply prop_right. intros. inversion H.
+  - simpl. sep_apply IHl. Intros. unfold node_rep at 2. Intros. apply prop_right.
+    intros. destruct H2.
+    + subst a. now split.
+    + now apply H.
+Qed.
 
 Definition lookup_inv (root: TreeNode) (b: val) (l: list TreeNode)
            (Cpc : pc_flowint) (Cs: bst_inset_flowint) (x: Z): environ -> mpred :=
   EX n: TreeNode, EX l': list TreeNode, EX nI: pc_flowint, EX Cl: pc_flowint,
   EX nS: bst_inset_flowint, EX Cls: bst_inset_flowint,
-    PROP (intJoin nI Cl Cpc; intJoin nS Cls Cs; in_inset x nS n;
+    PROP (intJoin nI Cl Cpc; intJoin nS Cls Cs;
          if Val.eq (addr_tn n) nullval
-         then nI = ∅ /\ nS = ∅ /\ l' = l /\ Cl = Cpc /\ Cls = Cs
-         else Permutation (n :: l') l)
+         then nI = ∅ /\ nS = ∅ /\ l' = l /\ Cl = Cpc /\ Cls = Cs /\
+              ~ In x (map key_tn l)
+         else in_inset x nS n /\ Permutation (n :: l') l)
     LOCAL (temp _p (addr_tn n); temp _t b; temp _x (Vint (Int.repr x)))
     SEP (data_at Tsh (tptr t_struct_tree) (addr_tn root) b;
         if Val.eq (addr_tn n) nullval then emp else node_rep n nI nS;
@@ -224,7 +287,8 @@ Lemma body_lookup: semax_body Vprog Gprog f_lookup lookup_spec.
 Proof.
   start_function.
   unfold treebox_rep. Intros. sep_apply (tree_rep_has_children root l Cpc Cs); auto.
-  Intros. forward.
+  Intros. sep_apply (tree_rep_root_no_parent root); auto. Intros. rename H4 into Hr.
+  forward.
   - entailer. sep_apply (tree_rep_saturate_local root l Cpc Cs); auto. entailer !.
   - forward_while (lookup_inv root b l Cpc Cs x).
     + Exists root. destruct H1 as [_ [_ [_ [? _]]]].
@@ -238,9 +302,8 @@ Proof.
     + if_tac.
       * Intros. subst. rewrite H4. entailer !.
       * sep_apply node_rep_valid_ptr. Intros. entailer !.
-    + if_tac. 1: now exfalso. unfold node_rep. Intros.
-      assert (In n l). {
-        eapply Permutation_in; eauto. now left. }
+    + if_tac. 1: now exfalso. unfold node_rep. Intros. destruct H6.
+      assert (In n l). { eapply Permutation_in; eauto. now left. }
       assert (data_at Tsh t_struct_tree
                       (Vint (Int.repr (key_tn n)),
                        (value_tn n, (left_tn n, right_tn n))) (addr_tn n) *
@@ -252,17 +315,58 @@ Proof.
         -- rewrite H3. entailer !.
         -- rewrite H16. sep_apply (tree_rep_is_ptr_null p l Cpc Cs). entailer !.
         -- admit.
-        -- admit.
+        -- rewrite H16. sep_apply (tree_rep_neq_nullval p l Cpc Cs). Intros.
+           rewrite (tree_rep_In_eq p l Cpc Cs); auto. Intros pI pS pl pClpc pCls.
+           Exists (p, pl, pI, pClpc, pS, pCls). simpl fst. simpl snd. if_tac.
+           1: now exfalso. unfold node_rep. Intros. unfold tree_rep at 1.
+           Intros fpc fs. sep_apply tree_rep_local_inv. Intros. rename H28 into Hl.
+           entailer !.
+           ++ destruct H9 as [? [? [? [? [? [? [? ?]]]]]]].
+              rewrite Int.signed_repr in H14; auto. destruct H8 as [? [? [? ?]]].
+              specialize (H42 p). unfold inset_edgeFn in H42. red.
+              rewrite <- H16 in H42. rewrite <- val_eqb_false in H33.
+              rewrite H33 in H42. rewrite <- H16 in H17.
+              rewrite <- val_eqb_false in H17. rewrite H17 in H42. simpl in H42.
+              rewrite val_eqb_refl in H42. red in H6. apply nzmap_elem_of_dom in H6.
+              red in H6. assert (p ≠ root). {
+                intro. subst p. destruct (Hr _ H11). auto. }
+              destruct H6 as [a ?].
+              assert (x ∈ dom_ms (out nS p)). {
+                rewrite nzmap_elem_of_dom. exists a. rewrite H42.
+                apply split_left_lookup. now split. } rename H44 into Hi.
+              assert (inf pS p = out nS p). {
+                destruct H2 as [[? ?] [? ?]]. destruct H22 as [_ [? _]].
+                pose proof (intJoin_unfold_inf_1 _ _ _ H19 H2 p).
+                assert (p ∈ domm pS). {
+                  rewrite H22. now apply elem_of_singleton_2. } specialize (H47 H48).
+                pose proof (intJoin_dom _ _ _ H19 H2).
+                assert (p ∈ domm Cs). {
+                  rewrite H49. rewrite elem_of_union. now left. }
+                rewrite H46 in H47; auto. rewrite ccm_left_id in H47.
+                assert (✓ pCls) by (apply (intJoin_valid_proj2 _ _ _ H19); auto).
+                assert (p ∉ domm pCls). {
+                  assert (intComposable pS pCls) by
+                      (eapply intComposable_valid; eauto).
+                  destruct H52 as [_ [_ [? _]]]. intro. now apply (H52 p). }
+                rewrite (list_join_unfold_out _ _ H25 H51 _ H52) in H47.
+                admit. }
+              admit.
+           ++ unfold tree_rep. Exists fpc fs. entailer !.
       * forward_if.
         -- forward; sep_apply H12; destruct H13 as [? | [p [? [? ?]]]].
            ++ rewrite H13; entailer !.
            ++ rewrite H17. sep_apply (tree_rep_is_ptr_null p l Cpc Cs). entailer !.
            ++ admit.
-           ++ admit.
-        -- forward; destruct H10 as [? [? [? [? [? [? [? ?]]]]]]].
+           ++ rewrite H17. sep_apply (tree_rep_neq_nullval p l Cpc Cs). Intros.
+           rewrite (tree_rep_In_eq p l Cpc Cs); auto. Intros pI pS pl pClpc pCls.
+           Exists (p, pl, pI, pClpc, pS, pCls). simpl fst. simpl snd. if_tac.
+           1: now exfalso. entailer !. admit.
+        -- forward; destruct H9 as [? [? [? [? [? [? [? ?]]]]]]].
            ++ entailer !.
            ++ sep_apply H12. forward. Exists (value_tn n). unfold treebox_rep.
               entailer !. right. exists n. split; [|split]; auto.
               rewrite Int.signed_repr in H14, H15; auto. lia.
-    + if_tac. 2: now exfalso.
+    + if_tac. 2: now exfalso. forward. Exists nullval.
+      destruct H6 as [? [? [? [? [? ?]]]]]. entailer !. unfold treebox_rep.
+      entailer !.
 Abort.
