concurrency/flows.v
@@ -7,7 +7,7 @@
 
 (*From iris.heap_lang Require Import proofmode.*)
 Require Export VST.veric.bi.
-Require Import VST.progs.ghosts.
+Require Import VST.concurrency.ghosts.
 
 From stdpp Require Export gmap.
 From stdpp Require Import mapset finite.
